intermed version where oracle is a single partrec fun

Computability/Encoding.lean
@@ -28,23 +28,21 @@ inductive codeo : Type
 | succ : codeo
 | left : codeo
 | right : codeo
-| oracle : ℕ → codeo
+| oracle : codeo
 | pair : codeo → codeo → codeo
 | comp : codeo → codeo → codeo
 | prec : codeo → codeo → codeo
 | rfind' : codeo → codeo
 
 
+
 /-- Semantics of `codeo`, relative to an indexed oracle family. -/
-def evalo {α : Type} [Primcodable α] (f : α → ℕ →. ℕ) : codeo → ℕ →. ℕ
+def evalo (f : ℕ →. ℕ) : codeo → ℕ →. ℕ
 | codeo.zero => pure 0
 | codeo.succ => fun n => some (n + 1)
 | codeo.left => fun n => some (Nat.unpair n).1
 | codeo.right => fun n => some (Nat.unpair n).2
-| codeo.oracle i =>
-    match decode i with
-    | some a => f a
-    | none   => λ n => ⊥
+| codeo.oracle => f
 | codeo.pair cf cg =>
     fun n => Nat.pair <$> evalo f cf n <*> evalo f cg n
 | codeo.comp cf cg =>
@@ -63,7 +61,7 @@ def encodeCodeo : codeo → ℕ
 | codeo.succ        => 1
 | codeo.left        => 2
 | codeo.right       => 3
-| codeo.oracle i    => 8 * i + 4
+| codeo.oracle      => 4
 | codeo.pair cf cg  => 8 * Nat.pair (encodeCodeo cf) (encodeCodeo cg) + 5
 | codeo.comp cf cg  => 8 * Nat.pair (encodeCodeo cf) (encodeCodeo cg) + 6
 | codeo.prec cf cg  => 8 * Nat.pair (encodeCodeo cf) (encodeCodeo cg) + 7
@@ -75,7 +73,7 @@ def decodeCodeo : ℕ → codeo
   | 1 => codeo.succ
   | 2 => codeo.left
   | 3 => codeo.right
-  | 4 => codeo.oracle 0
+  | 4 => codeo.oracle
   | n + 5 =>
     let m := (n + 5) / 8
     have hm : m < n + 5 := by
@@ -86,7 +84,7 @@ def decodeCodeo : ℕ → codeo
     have _m2 : m.unpair.2 < n + 5 := lt_of_le_of_lt m.unpair_right_le hm
     match (n + 5) % 8 with
     | 0 => codeo.rfind' (decodeCodeo m)
-    | 4 => codeo.oracle m
+    | 4 => codeo.oracle
     | 5 => codeo.pair (decodeCodeo m.unpair.1) (decodeCodeo m.unpair.2)
     | 6 => codeo.comp (decodeCodeo m.unpair.1) (decodeCodeo m.unpair.2)
     | 7 => codeo.prec (decodeCodeo m.unpair.1) (decodeCodeo m.unpair.2)
@@ -128,7 +126,7 @@ def const_inj : ∀ {n₁ n₂}, const n₁ = const n₂ → n₁ = n₂
     injection h with h₁ h₂
     simp only [const_inj h₂]
 
-theorem evalo_const {α : Type} [Primcodable α] (g : α → ℕ →. ℕ) : evalo g (const a) _b = a := by sorry
+theorem evalo_const (g : ℕ →. ℕ) : evalo g (const a) _b = a := by sorry
 
 /-- A code for the identity function. -/
 def id_code : codeo :=
@@ -140,9 +138,9 @@ def curry (c : codeo) (n : ℕ) : codeo :=
   codeo.comp c (codeo.pair (const n) id_code)
 
 -- -- helper lemma to prove rfind' case of univ theorem, since rfind' is defined differently from rfind
-theorem rfind'o {α : Type} [Primcodable α] {g : α → ℕ →. ℕ} {cf : codeo}
-    (hf : RecursiveIn (Set.range g) (evalo g cf)) :
-  RecursiveIn (Set.range g)
+theorem rfind'o {g : ℕ →. ℕ} {cf : codeo}
+    (hf : RecursiveIn g (evalo g cf)) :
+  RecursiveIn g
     (Nat.unpaired fun a m =>
       (Nat.rfind fun n =>
         (fun m => m = 0) <$> evalo g cf (Nat.pair a (n + m))
@@ -151,8 +149,8 @@ theorem rfind'o {α : Type} [Primcodable α] {g : α → ℕ →. ℕ} {cf : cod
 
 /-- A function is partial recursive relative to an indexed set of oracles `O` if and only if there is a code implementing it.
 Therefore, `evalo` is a **universal partial recursive function relative to `g`**. -/
-theorem exists_code_rel {α : Type} [Primcodable α] (g : α → ℕ →. ℕ) (f : ℕ →. ℕ) :
-  RecursiveIn (Set.range g) f ↔ ∃ c : codeo, evalo g c = f := by
+theorem exists_code_rel (g : ℕ →. ℕ) (f : ℕ →. ℕ) :
+  RecursiveIn g f ↔ ∃ c : codeo, evalo g c = f := by
   constructor
   · intro gf
     induction gf
@@ -160,12 +158,13 @@ theorem exists_code_rel {α : Type} [Primcodable α] (g : α → ℕ →. ℕ) (
     · exact ⟨codeo.succ, rfl⟩
     · exact ⟨codeo.left, rfl⟩
     · exact ⟨codeo.right, rfl⟩
-    · case mp.oracle hf =>
-      rcases hf with ⟨cf, rfl⟩
-      exact ⟨codeo.oracle (encode cf), by
-        funext n
-        simp only [evalo, codeo.oracle]
-        rw [encodek]⟩
+    · sorry
+    -- · case mp.oracle hf =>
+    --   rcases hf with ⟨cf, rfl⟩
+    --   exact ⟨codeo.oracle (encode cf), by
+    --     funext n
+    --     simp only [evalo, codeo.oracle]
+    --     rw [encodek]⟩
     · case mp.pair hf hg =>
       rcases hf with ⟨cf, rfl⟩; rcases hg with ⟨cg, rfl⟩
       exact ⟨codeo.pair cf cg, rfl⟩
@@ -190,17 +189,8 @@ theorem exists_code_rel {α : Type} [Primcodable α] (g : α → ℕ →. ℕ) (
       exact RecursiveIn.left
     | right =>
       exact RecursiveIn.right
-    | oracle i =>
-      cases h : decode (α := α) i with
-      | some a =>
-        apply RecursiveIn.of_eq (RecursiveIn.oracle (g a) (Set.mem_range_self _))
-        intro n
-        simp [evalo, h]
-      | none =>
-        apply RecursiveIn.of_eq RecursiveIn.none
-        intro n
-        simp [evalo, h]
-        rfl
+    | oracle =>
+      exact RecursiveIn.oracle
     | pair cf cg pf pg =>
       exact pf.pair pg
     | comp cf cg pf pg =>
